



Representation of solution of a Riemann–Liouville fractional differential equation with pure delay[☆]



Mengmeng Li^a, JinRong Wang^{a,b,*}

^a Department of Mathematics, Guizhou University, Guiyang, Guizhou 550025, China

^b School of Mathematical Sciences, Qufu Normal University, Qufu, Shandong 273165, China

ARTICLE INFO

Article history:

Received 11 April 2018

Accepted 5 June 2018

Available online 15 June 2018

Keywords:

Linear delay differential equation

Riemann–Liouville fractional

derivative

Delayed Mittag-Leffler type matrix

function

Solution

ABSTRACT

This paper derives a representation of a solution to the initial value problem for a linear fractional delay differential equation with Riemann–Liouville derivative. We apply the method of variation of constants to obtain the representation of a solution via a delayed Mittag-Leffler type matrix function.

© 2018 Published by Elsevier Ltd.

1. Introduction

Recently, Khusainov and Shuklin [1] and Diblík and Khusainov [2,3] introduce a new concept, delayed exponential matrix function, which is used to seek a representation of a solution to a linear time-invariant continuous/discrete delay equation. For more contributions of the representation of solutions, the stability, and the control theory for linear time-invariant continuous/discrete delay systems, we refer to [4–9] and the references.

Inspired by [7,8], we seek a representation of a solution to a linear fractional delay differential equation with Riemann–Liouville derivative whose the initial condition involving a singular kernel that is different from the standard initial condition for a Caputo fractional delay differential equation.

In this paper, we study a fractional delay differential equation of the form:

$$\begin{cases} (\mathbb{D}_{-\tau+}^{\alpha} y)(x) = By(x - \tau) + f(x), & B \in \mathbb{R}^{n \times n}, x \in (0, T], \tau > 0, \\ y(x) = \omega(x), & \omega(x) \in \mathbb{R}^n, -\tau \leq x \leq 0, \\ (\mathbb{I}_{-\tau+}^{1-\alpha} y)(-\tau^+) = \omega(-\tau), & \omega(-\tau) \in \mathbb{R}^n, \end{cases} \quad (1)$$

[☆] This work was supported by the National Natural Science Foundation of China (11661016), Training Object of High Level and Innovative Talents of Guizhou Province ((2016)4006) and Science and Technology Program of Guizhou Province ([2017]5788).

* Corresponding author at: Department of Mathematics, Guizhou University, Guiyang, Guizhou 550025, China.

E-mail addresses: Lmm0424@126.com (M. Li), jrwang@gzu.edu.cn (J. Wang).

where $\mathbb{D}_{-\tau+}^\alpha y$ denotes the Riemann–Liouville derivative of order $\alpha \in (0, 1)$ (see Definition 2.1), $\mathbb{I}_{-\tau+}^{1-\alpha} y$ denotes the Riemann–Liouville fractional integral of order $1 - \alpha$ (see Definition 2.2), $T = k^* \tau$ for a fixed $k^* \in \mathbb{N}^+ := \{1, 2, \dots\}$, τ is a fixed delay time, $f \in C([-\tau, T], \mathbb{R}^n)$, and ω is an arbitrary Riemann–Liouville differentiable vector function, i.e., $\mathbb{D}_{-\tau+}^\alpha \omega$ exists.

The main contributions are stated as follows.

We find a fundamental matrix for homogeneous problem of (3) and then derive its general solution. Next, we derive a special solution for (1) with zero initial condition. Finally, we give a representation of a solution of (1) via the superposition principle.

2. Preliminaries

Let $a, b \in \mathbb{R}, a < b$ and $C((a, b], \mathbb{R}^n)$ be the Banach space of vector-valued continuous function from $(a, b]$ into \mathbb{R}^n . Let Θ and I be the zero and identity matrices, respectively.

We recall some definitions and lemmas as follows.

Definition 2.1 (See [10]). The Riemann–Liouville derivative of order $0 < \alpha < 1$ for a function $f : [a, \infty) \rightarrow \mathbb{R}$ can be written as $(\mathbb{D}_{a+}^\alpha y)(x) = \frac{1}{\Gamma(1-\alpha)} \frac{d}{dx} \int_a^x (x-t)^{-\alpha} y(t) dt, x > a$.

Definition 2.2 (See [10]). The Riemann–Liouville fractional integral of order $0 < \alpha < 1$ for a function $f : [a, \infty) \rightarrow \mathbb{R}$ can be written as $(\mathbb{I}_{a+}^\alpha y)(x) = \frac{1}{\Gamma(\alpha)} \int_a^x (x-t)^{\alpha-1} y(t) dt, x > a$.

Definition 2.3 (See [7, Definition 2.5]). Set $0 < \alpha < 1$ and $\beta > 0$. Delayed two parameters Mittag-Leffler type matrix $\mathbb{Z}_{\tau, \beta}^{B, \alpha} : \mathbb{R} \rightarrow \mathbb{R}^{n \times n}$ is defined by

$$\mathbb{Z}_{\tau, \beta}^{B, \alpha} = \begin{cases} \Theta, & -\infty < x \leq -\tau, \\ I \frac{(\tau+x)^{\alpha-1}}{\Gamma(\beta)}, & -\tau < x \leq 0, \\ I \frac{(\tau+x)^{\alpha-1}}{\Gamma(\beta)} + B \frac{x^{2\alpha-1}}{\Gamma(\alpha+\beta)} + B^2 \frac{(x-\tau)^{3\alpha-1}}{\Gamma(2\alpha+\beta)} + \dots + B^k \frac{(x-(k-1)\tau)^{(k+1)\alpha-1}}{\Gamma(k\alpha+\beta)}, & (k-1)\tau < x \leq k\tau, k \in \mathbb{N}^+. \end{cases} \quad (2)$$

Lemma 2.4 (See [7, Lemma 2.6]). For any $(k-1)\tau < x \leq k\tau$, $0 \leq s \leq t$ and $k \in \mathbb{N}^+$ is a fixed number, we have $\int_{(k-1)\tau+s}^x (x-t)^{-\alpha} (t-(k-1)\tau-s)^{k\alpha-1} dt = (x-(k-1)\tau-s)^{(k-1)\alpha} \mathbb{B}[1-\alpha, k\alpha]$, where $\mathbb{B}[\xi, \eta] = \int_0^1 s^{\xi-1} (1-s)^{\eta-1} ds$ is a Beta function.

Lemma 2.5 (See [8, Lemma 2.5]). For any $(k-1)\tau < x \leq k\tau$ and $k \in \mathbb{N}^+$, we have $\int_{(k-1)\tau}^x (x-t)^{-\alpha} (t-(k-1)\tau)^{(k+1)\alpha-1} dt = (x-(k-1)\tau)^{k\alpha} \mathbb{B}[1-\alpha, (k+1)\alpha]$.

Lemma 2.6. Let $(k-1)\tau < x \leq k\tau$, $-\tau \leq s \leq t$ and $k \in \mathbb{N}^+$ is a fixed number, we have $\int_s^x (x-t)^{-\alpha} \mathbb{Z}_{\tau, \alpha}^{B, (t-\tau-s)^\alpha} dt = \sum_{i=0}^k \int_{i\tau+s}^x (x-t)^{-\alpha} B^i \frac{(t-i\tau-s)^{(i+1)\alpha-1}}{\Gamma(i\alpha+\alpha)} dt$.

Proof. The proof is similar to [7, Lemma 2.7], so we omit it here. \square

3. Main results

Firstly, we use (2) to construct the explicit formula of solutions of

$$\begin{cases} (\mathbb{D}_{-\tau+}^\alpha y)(x) = By(x - \tau), \quad y(x) \in \mathbb{R}^n, \quad x \in (0, T], \quad \tau > 0, \\ y(x) = \omega(x), \quad \omega(x) \in \mathbb{R}^n \quad -\tau \leq x \leq 0, \\ (\mathbb{I}_{-\tau+}^{1-\alpha} y)(-\tau^+) = \omega(-\tau), \quad \omega(-\tau) \in \mathbb{R}^n. \end{cases} \quad (3)$$

Theorem 3.1. For delayed Mittag-Leffler type matrix $\mathbb{Z}_{\tau,\alpha}^{B,\alpha} : \mathbb{R} \rightarrow \mathbb{R}^{n \times n}$, one has $(\mathbb{D}_{-\tau+}^\alpha \mathbb{Z}_{\tau,\alpha}^{Bt^\alpha})(x) = B\mathbb{Z}_{\tau,\alpha}^{B(x-\tau)^\alpha}$, i.e., $\mathbb{Z}_{\tau,\alpha}^{Bx^\alpha}$ is a solution of $(\mathbb{D}_{-\tau+}^\alpha y)(x) = By(x - \tau)$, that satisfies initial conditions $\mathbb{Z}_{\tau,\alpha}^{Bx^\alpha} = I \frac{(\tau+x)^{\alpha-1}}{\Gamma(\alpha)}$, $-\tau \leq x \leq 0$.

Proof. For $x \in ((k-1)\tau, k\tau]$ and $k \in \mathbb{N}^+$. We adopt the mathematical induction to prove our result.

(i) For $k = 1, 0 < x \leq \tau$, we have

$$y(x) = \mathbb{Z}_{\tau,\alpha}^{Bx^\alpha} = I \frac{(\tau+x)^{\alpha-1}}{\Gamma(\alpha)} + B \frac{x^{2\alpha-1}}{\Gamma(\alpha+\alpha)}. \quad (4)$$

By using Definition 2.1 for $\mathbb{Z}_{\tau,\alpha}^{B,\alpha}$ via (4) and Lemma 2.5, we obtain

$$\begin{aligned} (\mathbb{D}_{-\tau+}^\alpha \mathbb{Z}_{\tau,\alpha}^{Bt^\alpha})(x) &= \frac{1}{\Gamma(1-\alpha)} \frac{d}{dx} \left(\int_{-\tau}^0 (x-t)^{-\alpha} y(t) dt + \int_0^x (x-t)^{-\alpha} y(t) dt \right) \\ &= \frac{1}{\Gamma(1-\alpha)} \frac{d}{dx} \left(\int_{-\tau}^x (x-t)^{-\alpha} I \frac{(\tau+t)^{\alpha-1}}{\Gamma(\alpha)} dt + \int_0^x (x-t)^{-\alpha} B \frac{t^{2\alpha-1}}{\Gamma(\alpha+\alpha)} dt \right) \\ &= \frac{1}{\Gamma(1-\alpha)} \frac{d}{dx} \left(I \frac{\mathbb{B}[1-\alpha, \alpha]}{\Gamma(\alpha)} + \frac{B}{\Gamma(2\alpha)} x^\alpha \mathbb{B}[1-\alpha, 2\alpha] \right) = B \frac{x^{\alpha-1}}{\Gamma(\alpha)}. \end{aligned}$$

(ii) For $k = 2, \tau < x \leq 2\tau$, we have

$$y(x) = \mathbb{Z}_{\tau,\alpha}^{Bx^\alpha} = I \frac{(\tau+x)^{\alpha-1}}{\Gamma(\alpha)} + B \frac{x^{2\alpha-1}}{\Gamma(\alpha+\alpha)} + B^2 \frac{(x-\tau)^{3\alpha-1}}{\Gamma(2\alpha+\alpha)}. \quad (5)$$

By using Definition 2.1 for $\mathbb{Z}_{\tau,\alpha}^{B,\alpha}$ via (5) and Lemma 2.5, we obtain

$$\begin{aligned} (\mathbb{D}_{-\tau+}^\alpha \mathbb{Z}_{\tau,\alpha}^{Bt^\alpha})(x) &= \frac{1}{\Gamma(1-\alpha)} \frac{d}{dx} \left(\int_{-\tau}^\tau (x-t)^{-\alpha} y(t) dt + \int_\tau^x (x-t)^{-\alpha} y(t) dt \right) \\ &= B \frac{x^{\alpha-1}}{\Gamma(\alpha)} + \frac{1}{\Gamma(1-\alpha)} \frac{d}{dx} \int_\tau^x (x-t)^{-\alpha} B^2 \frac{(t-\tau)^{3\alpha-1}}{\Gamma(2\alpha+\alpha)} dt \\ &= B \frac{x^{\alpha-1}}{\Gamma(\alpha)} + B^2 \frac{(x-\tau)^{2\alpha-1}}{\Gamma(2\alpha)}. \end{aligned}$$

(iii) Suppose $k = n, (n-1)\tau < x \leq n\tau$ and $n \in \mathbb{N}^+$, the following relation holds:

$$(\mathbb{D}_{-\tau+}^\alpha \mathbb{Z}_{\tau,\alpha}^{Bt^\alpha})(x) = B \frac{x^{\alpha-1}}{\Gamma(\alpha)} + B^2 \frac{(x-\tau)^{2\alpha-1}}{\Gamma(2\alpha)} + \cdots + B^n \frac{(x-(n-1)\tau)^{n\alpha-1}}{\Gamma(n\alpha)}.$$

Next, for $k = n+1, n\tau < x \leq (n+1)\tau$, we have

$$y(x) = \mathbb{Z}_{\tau,\alpha}^{Bx^\alpha} = I \frac{(\tau+x)^{\alpha-1}}{\Gamma(\alpha)} + B \frac{x^{2\alpha-1}}{\Gamma(\alpha+\alpha)} + \cdots + B^{n+1} \frac{(x-n\tau)^{(n+2)\alpha-1}}{\Gamma((n+1)\alpha+\alpha)}. \quad (6)$$

By using Definition 2.1 for $\mathbb{Z}_{\tau,\alpha}^{B,\alpha}$ via (6) and Lemma 2.5, we obtain

$$\begin{aligned} & (\mathbb{D}_{-\tau+}^{\alpha} \mathbb{Z}_{\tau,\alpha}^{Bt^{\alpha}})(x) \\ &= \frac{1}{\Gamma(1-\alpha)} \frac{d}{dx} \left(\int_{-\tau}^0 (x-t)^{-\alpha} y(t) dt + \int_0^{\tau} (x-t)^{-\alpha} y(t) dt + \cdots + \int_{n\tau}^x (x-t)^{-\alpha} y(t) dt \right) \\ &= B \frac{x^{\alpha-1}}{\Gamma(\alpha)} + B^2 \frac{(x-\tau)^{2\alpha-1}}{\Gamma(2\alpha)} + \cdots + B^n \frac{(x-(n-1)\tau)^{n\alpha-1}}{\Gamma(n\alpha)} \\ &\quad + \frac{1}{\Gamma(1-\alpha)} \frac{d}{dx} \left(\frac{B^{n+1}}{\Gamma((n+1)\alpha + \alpha)} \int_{n\tau}^x (x-t)^{-\alpha} (t-n\tau)^{(n+2)\alpha-1} dt \right) \\ &= B \frac{x^{\alpha-1}}{\Gamma(\alpha)} + B^2 \frac{(x-\tau)^{2\alpha-1}}{\Gamma(2\alpha)} + \cdots + B^{n+1} \frac{(x-n\tau)^{(n+1)\alpha-1}}{\Gamma((n+1)\alpha)}. \end{aligned}$$

Therefore, for any $(k-1)\tau < x \leq k\tau$ and $k \in \mathbb{N}^+$, according to the mathematical induction, we have

$$(\mathbb{D}_{-\tau+}^{\alpha} \mathbb{Z}_{\tau,\alpha}^{Bt^{\alpha}})(x) = B \left(\frac{x^{\alpha-1}}{\Gamma(\alpha)} + B \frac{(x-\tau)^{2\alpha-1}}{\Gamma(2\alpha)} + \cdots + B^{k-1} \frac{(x-(k-1)\tau)^{k\alpha-1}}{\Gamma(k\alpha)} \right) = B \mathbb{Z}_{\tau,\alpha}^{B(x-\tau)^{\alpha}}.$$

The proof is completed. \square

Theorem 3.2. Let $(n-1)\tau < x \leq n\tau$ for all $n \in \{0, 1, 2, \dots, k^*\}$. A solution $y \in C(X, \mathbb{R}^n)$ of (3) can be expressed by the following formula

$$y(x) = \mathbb{Z}_{\tau,\alpha}^{Bx^{\alpha}} \omega(-\tau) + \int_{-\tau}^0 \mathbb{Z}_{\tau,\alpha}^{B(x-\tau-s)^{\alpha}} (\mathbb{D}_{-\tau+}^{\alpha} \omega)(s) ds, \quad (7)$$

where either $X = ((n-1)\tau, n\tau]$ for $0 < \alpha < 1/(n+1)$ or $X = [(n-1)\tau, n\tau]$ for $\alpha \geq 1/(n+1)$.

Proof. Let matrix $Y_0(x) = \mathbb{Z}_{\tau,\alpha}^{Bx^{\alpha}}$ satisfy Theorem 3.1 and any solution of (3) satisfy initial conditions $y(x) = \omega(x)$, $-\tau \leq x \leq 0$ should search in the form

$$y(x) = Y_0(x)C + \int_{-\tau}^0 \mathbb{Z}_{\tau,\alpha}^{B(x-\tau-s)^{\alpha}} z(s) ds. \quad (8)$$

where C is a vector of unknown constant, $z(\cdot)$ is an unknown Riemann–Liouville differentiable vector function. According to the matrix $Y_0(x)$ is a solution of (3). Therefore, we choose C satisfying $(\mathbb{I}_{-\tau+}^{1-\alpha} y)(-\tau^+) = \omega(-\tau)$.

Let us assume $x = -\tau$, by using Definition 2.3, we obtain $\mathbb{Z}_{\tau,\alpha}^{B(-2\tau-s)^{\alpha}} = \Theta$ with $-\tau \leq s \leq 0$. For $-\tau < x \leq 0$, we have

$$\begin{aligned} \omega(-\tau) &= (\mathbb{I}_{-\tau+}^{1-\alpha} y)(-\tau^+) = \lim_{x \rightarrow -\tau^+} (\mathbb{I}_{-\tau+}^{1-\alpha} y)(x) \\ &= \lim_{x \rightarrow -\tau^+} \left(\frac{1}{\Gamma(1-\alpha)} \int_{-\tau}^x (x-t)^{-\alpha} Y_0(t) C dt \right) \\ &= \lim_{x \rightarrow -\tau^+} \frac{C}{\Gamma(1-\alpha)} \left(\int_{-\tau}^x (x-t)^{-\alpha} (\tau+t)^{\alpha-1} dt \right) = \lim_{x \rightarrow -\tau^+} C = C, \end{aligned}$$

which implied the formula (8) takes a form

$$y(x) = \mathbb{Z}_{\tau,\alpha}^{Bx^{\alpha}} \omega(-\tau) + \int_{-\tau}^0 \mathbb{Z}_{\tau,\alpha}^{B(x-\tau-s)^{\alpha}} z(s) ds.$$

Since $-\tau \leq x \leq 0$, one should divide interval into two subintervals, we have

(i) For $-\tau \leq s \leq x$, and $-\tau \leq x - \tau - s \leq x$, the delayed Mittag-Leffler type matrix $\mathbb{Z}_{\tau,\alpha}^{B(x-\tau-s)^\alpha} = I \frac{(x-s)^{\alpha-1}}{\Gamma(\alpha)}$.

(ii) For $x \leq s \leq 0$, and $x - \tau \leq x - \tau - s \leq -\tau$, the delayed Mittag-Leffler type matrix $\mathbb{Z}_{\tau,\alpha}^{B(x-\tau-s)^\alpha} = \Theta$. Thus on the interval $-\tau \leq x \leq 0$, we have

$$\omega(x) = I \frac{(\tau+x)^{\alpha-1}}{\Gamma(\alpha)} \omega(-\tau) + \int_{-\tau}^x I \frac{(x-s)^{\alpha-1}}{\Gamma(\alpha)} z(s) ds. \quad (9)$$

Having Riemann–Liouville fractional differentiation on both sides of (9), we have

$$\begin{aligned} (\mathbb{D}_{-\tau+}^\alpha \omega)(x) &= \frac{1}{\Gamma(1-\alpha)} \frac{d}{dx} \int_{-\tau}^x (x-t)^{-\alpha} \left(I \frac{(\tau+t)^{\alpha-1}}{\Gamma(\alpha)} \omega(-\tau) + \int_{-\tau}^t I \frac{(t-s)^{\alpha-1}}{\Gamma(\alpha)} z(s) ds \right) dt \\ &= \frac{I}{\Gamma(1-\alpha)} \frac{d}{dx} \int_{-\tau}^x \frac{z(s)}{\Gamma(\alpha)} \left(\int_s^x (x-t)^{-\alpha} (t-s)^{\alpha-1} dt \right) ds = \frac{d}{dx} \int_{-\tau}^x z(s) ds = z(x). \end{aligned}$$

The proof is completed. \square

Now we are ready to derive a special solution of (1) with the zero initial conditions.

Theorem 3.3. A solution $\tilde{y} \in C([-\tau, T], \mathbb{R}^n)$ of (1) satisfying initial conditions $y(x) = 0$, $x \in [-\tau, 0]$ has a form

$$\tilde{y}(x) = \int_{-\tau}^x \mathbb{Z}_{\tau,\alpha}^{B(x-\tau-t)^\alpha} f(t) dt, \quad x \in [0, T].$$

Proof. Having used method of variation of constants, solution of nonhomogeneous system $\tilde{y}(x)$ will be search in the form

$$\tilde{y}(x) = \int_{-\tau}^x \mathbb{Z}_{\tau,\alpha}^{B(x-\tau-t)^\alpha} c(t) dt, \quad (10)$$

where $c(\cdot)$, $-\tau \leq t \leq x$ is an unknown vector function and $\tilde{y}(0) = 0$.

Taking the Riemann–Liouville fractional differentiate for formula (10), we obtain

(i) For $k = 1$ and $0 < x \leq \tau$, according to (1), we have

$$\begin{aligned} (\mathbb{D}_{-\tau+}^\alpha \tilde{y})(x) &= B \tilde{y}(x - \tau) + f(x) = B \int_{-\tau}^{x-\tau} \mathbb{Z}_{\tau,\alpha}^{B(x-2\tau-t)^\alpha} c(t) dt + f(x) \\ &= B \int_{-\tau}^{x-\tau} I \frac{(x-\tau-t)^{\alpha-1}}{\Gamma(\alpha)} c(t) dt + f(x). \end{aligned}$$

However, according to Definition 2.1 and Lemma 2.6, we have

$$\begin{aligned} &(\mathbb{D}_{-\tau+}^\alpha \tilde{y})(x) \\ &= \frac{1}{\Gamma(1-\alpha)} \frac{d}{dx} \int_{-\tau}^x (x-t)^{-\alpha} \left(\int_{-\tau}^t \mathbb{Z}_{\tau,\alpha}^{B(t-\tau-s)^\alpha} c(s) ds \right) dt \\ &= \frac{1}{\Gamma(1-\alpha)} \frac{d}{dx} \int_{-\tau}^x c(s) \left(\int_s^x (x-t)^{-\alpha} \mathbb{Z}_{\tau,\alpha}^{B(t-\tau-s)^\alpha} dt \right) ds \\ &= \frac{1}{\Gamma(1-\alpha)} \frac{d}{dx} \int_{-\tau}^x c(s) \left(\int_s^x (x-t)^{-\alpha} I \frac{(t-s)^{\alpha-1}}{\Gamma(\alpha)} dt + \int_{\tau+s}^x (x-t)^{-\alpha} B \frac{(t-\tau-s)^{2\alpha-1}}{\Gamma(2\alpha)} dt \right) ds \\ &= \frac{d}{dx} \int_{-\tau}^x c(s) ds + \frac{1}{\Gamma(1-\alpha)} \frac{d}{dx} \int_{-\tau}^{x-\tau} c(s) \left(\int_{\tau+s}^x (x-t)^{-\alpha} B \frac{(t-\tau-s)^{2\alpha-1}}{\Gamma(2\alpha)} dt \right) ds \\ &= c(x) + \frac{B}{\Gamma(\alpha+1)} \frac{d}{dx} \int_{-\tau}^{x-\tau} c(s) (x-\tau-s)^\alpha ds = c(x) + B \int_{-\tau}^{x-\tau} \frac{(x-\tau-s)^{\alpha-1}}{\Gamma(\alpha)} c(s) ds. \end{aligned}$$

Hence, we obtain $c(x) = f(x)$.

(ii) For $(k-1)\tau < x \leq k\tau$ and $k \in \mathbb{N}^+$, according to (1), we have

$$\begin{aligned} (\mathbb{D}_{-\tau+}^\alpha \tilde{y})(x) &= B\tilde{y}(x-\tau) + f(x) = B \int_{-\tau}^{x-\tau} \mathbb{Z}_{\tau,\alpha}^{B(x-2\tau-t)^\alpha} c(t) dt + f(x) \\ &= \sum_{i=1}^k \int_{-\tau}^{x-i\tau} B^i \frac{(x-i\tau-t)^{i\alpha-1}}{\Gamma(i\alpha)} c(t) dt + f(x). \end{aligned}$$

However, according to Definition 2.1, we have

$$\begin{aligned} (\mathbb{D}_{-\tau+}^\alpha \tilde{y})(x) &= \frac{1}{\Gamma(1-\alpha)} \frac{d}{dx} \int_{-\tau}^x (x-t)^{-\alpha} \left(\int_{-\tau}^t \mathbb{Z}_{\tau,\alpha}^{B(t-\tau-s)^\alpha} c(s) ds \right) dt \\ &= \frac{1}{\Gamma(1-\alpha)} \frac{d}{dx} \int_{-\tau}^x c(s) \left(\int_s^x (x-t)^{-\alpha} \mathbb{Z}_{\tau,\alpha}^{B(t-\tau-s)^\alpha} dt \right) ds. \end{aligned}$$

According to Lemmas 2.4 and 2.6, we obtain

$$\begin{aligned} &(\mathbb{D}_{-\tau+}^\alpha \tilde{y})(x) \\ &= \frac{d}{dx} \int_{-\tau}^x c(s) ds + \sum_{i=1}^k \frac{1}{\Gamma(1-\alpha)} \frac{d}{dx} \int_{-\tau}^{x-i\tau} c(s) \left(\int_{i\tau+s}^x (x-t)^{-\alpha} B^i \frac{(t-i\tau-s)^{(i+1)\alpha-1}}{\Gamma(i\alpha+\alpha)} dt \right) ds \\ &= c(x) + \sum_{i=1}^k \frac{B^i}{\Gamma(i\alpha+1)} \frac{d}{dx} \int_{-\tau}^{x-i\tau} c(s) (x-i\tau-s)^{i\alpha} ds \\ &= c(x) + \sum_{i=1}^k \int_{-\tau}^{x-i\tau} B^i \frac{(x-i\tau-t)^{i\alpha-1}}{\Gamma(i\alpha)} c(t) dt. \end{aligned}$$

Hence, we obtain $c(x) = f(x)$. The proof is completed. \square

Linking Theorems 3.2 and 3.3 via the superposition principle, we have the following result.

Theorem 3.4. A solution $y \in C(X, \mathbb{R}^n) \cap C([-\tau, T], \mathbb{R}^n)$ of (1) satisfying initial conditions $y(x) = \omega(x)$, $-\tau \leq x \leq 0$ has a form

$$y(x) = \mathbb{Z}_{\tau,\alpha}^{Bx^\alpha} \omega(-\tau) + \int_{-\tau}^0 \mathbb{Z}_{\tau,\alpha}^{B(x-\tau-s)^\alpha} (\mathbb{D}_{-\tau+}^\alpha \omega)(s) ds + \int_{-\tau}^x \mathbb{Z}_{\tau,\alpha}^{B(x-\tau-t)^\alpha} f(t) dt.$$

Finally, an example is presented to illustrate the above theoretical results.

Let $\alpha = 0.3$, $\tau = 0.4$, $k^* = 4$ and $T = 1.6$. Consider

$$\begin{cases} \mathbb{D}_{0+}^{0.3} y(x) = By(x-0.4) + f(x), & x \in (0, 1.6], \\ \omega(x) = (0.1, 0.2)^\top, & -0.4 \leq x \leq 0, \\ (\mathbb{I}_{-0.4+}^{0.7} y)(-0.4^+) = \omega(-0.4), \end{cases} \quad (11)$$

where

$$y(x) = \begin{pmatrix} y_1(x) \\ y_2(x) \end{pmatrix}, \quad B = \begin{pmatrix} 0.2 & 0.1 \\ 0.3 & 0.5 \end{pmatrix}, \quad f(x) = \begin{pmatrix} x \\ x^2 \end{pmatrix}.$$

By Theorem 3.4, for every $x \in (0.4(k-1), 0.4k]$, $k \in \{1, 2, 3, 4\}$, the explicit solution of (11) can be expressed by

$$y(x) = \mathbb{Z}_{0.4,0.3}^{Bx^{0.3}} \omega(-0.4) + \int_{-0.4}^0 \mathbb{Z}_{0.4,0.3}^{B(x-0.4-s)^{0.3}} (\mathbb{D}_{-0.4+}^{0.3} \omega)(s) ds + \int_{-0.4}^x \mathbb{Z}_{0.4,0.3}^{B(x-0.4-t)^{0.3}} f(t) dt,$$

where

$$\begin{aligned} & \int_{-0.4}^0 \mathbb{Z}_{0.4,0.3}^{B(x-0.4-s)^{0.3}} (\mathbb{D}_{-0.4+}^{0.3} \omega)(s) ds \\ &= \frac{1}{\Gamma(0.7)} \int_{-0.4}^0 \mathbb{Z}_{0.4,0.3}^{B(x-0.4-s)^{0.3}} \left(\frac{d}{ds} \int_{-0.4}^s \left(\frac{0.1(s-t)^{-0.3}}{0.2(s-t)^{-0.3}} \right) dt \right) ds \\ &= \frac{1}{\Gamma(0.7)} \int_{-0.4}^0 \mathbb{Z}_{0.4,0.3}^{B(x-0.4-s)^{0.3}} \left(\frac{0.1(s+\tau)^{-0.3}}{0.2(s+\tau)^{-0.3}} \right) ds, \end{aligned}$$

and

$$\mathbb{Z}_{0.4,0.3}^{Bx^{0.3}} \varphi(-0.4) = \sum_{i=0}^k B^i \frac{(x - (i-1)0.4)^{0.3(i+1)-1}}{\Gamma((i+1)0.3)}, \quad k \in \{1, 2, 3, 4\}.$$

References

- [1] D.Ya. Khusainov, G.V. Shuklin, Linear autonomous time-delay system with permutation matrices solving, *Stud. Univ. žilina* 17 (2003) 101–108.
- [2] J. Diblík, D.Ya. Khusainov, Representation of solutions of discrete delayed system $x(k+1) = Ax(k) + Bx(k-m) + f(k)$ with commutative matrices, *J. Math. Anal. Appl.* 318 (2006) 63–76.
- [3] J. Diblík, D.Ya. Khusainov, Representation of solutions of linear discrete systems with constant coefficients and pure delay, *Adv. Difference Equ.* 2006 (2006) Art. ID 80825, 1–13.
- [4] D.Ya. Khusainov, J. Diblík, M. Růžicková, J. Lukáčová, Representation of a solution of the cauchy problem for an oscillating system with pure delay, *Nonlinear Oscil.* 11 (2008) 261–270.
- [5] J. Diblík, M. Fečkan, M. Pospíšil, Representation of a solution of the cauchy problem for an oscillating system with two delays and permutable matrices, *Ukrainian Math. J.* 65 (2013) 58–69.
- [6] M. Medved, M. Pospíšil, Sufficient conditions for the asymptotic stability of nonlinear multidelay differential equations with linear parts defined by pairwise permutable matrices, *Nonlinear Anal.* 75 (2012) 3348–3363.
- [7] M. Li, J. Wang, Exploring delayed Mittag-Leffler type matrix functions to study finite time stability of fractional delay differential equations, *Appl. Math. Comput.* 324 (2018) 254–265.
- [8] M. Li, J. Wang, Finite time stability of fractional delay differential equations, *Appl. Math. Lett.* 64 (2017) 170–176.
- [9] C. Liang, J. Wang, D. O'Regan, Representation of solution of a fractional linear system with pure delay, *Appl. Math. Lett.* 77 (2018) 72–78.
- [10] A.A. Kilbas, H.M. Srivastava, J.J. Trujillo, *Theory and Applications of Fractional Differential Equations*, Elsevier Science B.V., 2006.